theories/Borda_Rule_Ref.thy
@@ -6,6 +6,7 @@ begin
 
 definition borda_rule_sep where
   "borda_rule_sep \<equiv> elector_sep borda_elim_sep"
+
                                    
 interpretation borda_rule_impl: elector_sepref borda_ref borda_elim_sep borda
   apply unfold_locales            
@@ -14,19 +15,17 @@ interpretation borda_rule_impl: elector_sepref borda_ref borda_elim_sep borda
   subgoal apply (intro frefI) using borda_ref_correct[THEN frefD] by auto
   done
 
-lemmas borda_rule_correct_aux [sepref_comb_rules] = borda_rule_impl.elector_sep_correct
-
-lemma  borda_rule_correct:
+lemma  borda_rule_correct [sepref_fr_rules]:
   shows "(uncurry borda_rule_sep, uncurry (RETURN oo borda_rule))
     \<in> [\<lambda>(A, pl).
            finite_profile A
             pl]\<^sub>a (hr_comp (hs.assn id_assn) (\<langle>Id\<rangle>set_rel))\<^sup>k *\<^sub>a
                   (list_assn
-                    (hr_comp ballot_impl_assn
+                    (hr_comp (ballot_impl_assn id_assn)
                       ballot_rel))\<^sup>k \<rightarrow> hr_comp (hs.assn id_assn) (\<langle>Id\<rangle>set_rel) \<times>\<^sub>a
                                         hr_comp (hs.assn id_assn) (\<langle>Id\<rangle>set_rel) \<times>\<^sub>a
                                         hr_comp (hs.assn id_assn) (\<langle>Id\<rangle>set_rel)"
-  unfolding borda_rule_sep_def borda_rule.simps using borda_rule_correct_aux .
+  unfolding borda_rule_sep_def borda_rule.simps using borda_rule_impl.elector_sep_correct .
 
 
 export_code borda_rule_sep in Scala_imp
