theories/Compositional_Structures/Basic_Modules/Condorcet_Module_Ref.thy
@@ -67,8 +67,8 @@ qed
 
 sepref_definition condorcet_elim_sep is
   "uncurry condorcet_ref":: 
-  "alts_set_impl_assn\<^sup>k *\<^sub>a profile_impl_assn\<^sup>k 
-   \<rightarrow>\<^sub>a (result_impl_assn)"
+  "(alts_set_impl_assn id_assn)\<^sup>k *\<^sub>a (profile_impl_assn id_assn)\<^sup>k 
+   \<rightarrow>\<^sub>a (result_impl_assn id_assn)"
   unfolding condorcet_ref_def  max_eliminator_ref_def condorcet_score_ref_def 
     less_eliminator_ref_def  elimination_module_ref_def[abs_def] eliminate_def[abs_def]
     pre_compute_scores_def[abs_def] scoremax_def[abs_def] 
