theories/Compositional_Structures/Sepref_Bindings.thy
@@ -3,6 +3,7 @@ theory Sepref_Bindings
     "Basic_Modules/Condorcet_Module_Ref"  
     "Basic_Modules/Component_Types/Defer_Equal_Condition_Ref"
     Sequential_Composition_Ref
+    "../Borda_Rule_Ref"
 
 begin
 
@@ -25,8 +26,12 @@ lemma condorcet_aux:
   done
 
 
-sepref_decl_op (no_def) "borda :: 'a Electoral_Module" :: "elec_mod_rel_orig Id" 
-  using borda_aux .
+sepref_decl_op  (no_def) borda ::  "elec_mod_rel_orig R" where "R = Id"
+    apply standard
+  apply (rule nres_relI)
+  apply simp done
+
+
 
 
 sepref_decl_op (no_def) defer_equal_imp: "(defer_equal_condition)" :: 
@@ -37,18 +42,18 @@ sepref_decl_op (no_def) defer_equal_imp: "(defer_equal_condition)" ::
 
                               
 
-definition "alts_ref_assn \<equiv> hr_comp alts_set_impl_assn (\<langle>Id\<rangle>set_rel)"
+definition "alts_ref_assn \<equiv> hr_comp (alts_set_impl_assn id_assn) (\<langle>Id\<rangle>set_rel)"
                                  
 
-definition "ballot_ref_assn \<equiv>  hr_comp (ballot_impl_assn) (\<langle>Id\<rangle>list_rel)"
+definition "ballot_ref_assn \<equiv>  hr_comp (ballot_impl_assn id_assn) (\<langle>Id\<rangle>list_rel)"
 
 definition "alts_assn \<equiv> hr_comp alts_ref_assn (\<langle>Id\<rangle>set_rel)"
-
-definition "result_set_one_step \<equiv> hr_comp alts_set_impl_assn (\<langle>Id\<rangle>set_rel)"
+                                           
+definition "result_set_one_step \<equiv> hr_comp (alts_set_impl_assn id_assn) (\<langle>Id\<rangle>set_rel)"
 
 definition "result_set_assn \<equiv> hr_comp(result_set_one_step) (\<langle>Id\<rangle>set_rel)"
 
-definition "ballot_assn \<equiv> hr_comp (hr_comp (ballot_impl_assn) ballot_rel) (\<langle>Id \<times>\<^sub>r Id\<rangle>set_rel)"
+definition "ballot_assn \<equiv> hr_comp (hr_comp (ballot_impl_assn id_assn) ballot_rel) (\<langle>Id \<times>\<^sub>r Id\<rangle>set_rel)"
 
 
 locale refine_assns =
@@ -58,27 +63,41 @@ locale refine_assns =
        alts_ref_assn_def[symmetric,fcomp_norm_unfold] 
        ballot_ref_assn_def[symmetric,fcomp_norm_unfold]
        alts_assn_def[symmetric,fcomp_norm_unfold] 
-       result_set_one_step_def[symmetric,fcomp_norm_unfold]
       
 begin
 
 
-sepref_decl_impl borda_impl: borda_elim_sep.refine[FCOMP borda_ref_correct] 
-  by simp                                       
+sepref_decl_impl borda : borda_elim_sep.refine[FCOMP borda_ref_correct] 
+  by simp                                                              
 
-         
+definition "dimpls \<equiv> op_borda {1::nat, 2} [{(1::nat, 2)}]"
 
-sepref_decl_impl defer_eqal_condition_impl: defer_equal_condition_sep.refine .
-
- definition "funsc A p \<equiv> RETURN (borda A p)"
-
- sepref_definition first_imple 
-    is "uncurry funsc" :: "unit_assn\<^sup>k \<rightarrow>\<^sub>a  (alts_assn \<times>\<^sub>a alts_assn \<times>\<^sub>a alts_assn) "
-   unfolding funsc_def id_def comp_def
+ sepref_definition second_imple 
+    is "uncurry0 (RETURN dimpls)" ::
+ "unit_assn\<^sup>k \<rightarrow>\<^sub>a (result_impl_assn nat_assn)"
+   unfolding  dimpls_def comp_def
+   apply (rewrite in "op_borda rewrite_HOLE _" hs.fold_custom_empty)
+   apply (rewrite in "_ # rewrite_HOLE" HOL_list.fold_custom_empty)
+   unfolding hs.fold_custom_empty
    apply sepref_dbg_keep
+apply sepref_dbg_trans_keep
+   done
 
 
 end
+
+
+definition "impls \<equiv> borda_ref {1::nat, 2} ((([] @ [1::nat])@ [2::nat]) # [])"
+
+ sepref_definition first_imple 
+    is "uncurry0 (impls)" ::
+ "unit_assn\<^sup>k \<rightarrow>\<^sub>a (result_impl_assn nat_assn)"
+   unfolding  impls_def comp_def
+   apply (rewrite in "borda_ref rewrite_HOLE _" hs.fold_custom_empty)
+   apply (rewrite in "[(rewrite_HOLE @ [1::nat])@ [2::nat]]" arl.fold_custom_empty)
+   apply (rewrite in "_ # rewrite_HOLE" HOL_list.fold_custom_empty)
+   apply sepref_dbg_keep
+   done
 
 
 
